deps/poulet4/lib/P4cub/Transformations/Lifting/Lifted.v
@@ -106,11 +106,9 @@ Section Lifted.
       lifted_expr e ->
       lifted_expr <{ Access e[z] : ts @ i }>.
 
-  Inductive lifted_args : Expr.arrowE tags_t -> Prop :=
-  | lifted_args_arrow tes teo :
-      F.predfs_data (pred_paramarg_same lifted_expr) tes ->
-      predop lifted_expr teo ->
-      lifted_args (Arrow tes teo).
+  Definition lifted_args (args : Expr.arrowE tags_t) : Prop :=
+    F.predfs_data (pred_paramarg_same lifted_expr) (paramargs args) /\
+    predop lifted_expr (rtrns args).
   
   Inductive lifted_stmt : Stmt.s tags_t -> Prop :=
   | lifted_skip i :
@@ -195,32 +193,33 @@ Section Lifted.
       lifted_expr e -> lifted_stmt (Stmt.SSetValidity e validity i).
   
   Local Hint Constructors lifted_expr : core.
-  (*Print Field.predfs_data.*)
+
   Inductive lifted_parser_expr : Parser.e tags_t -> Prop :=
   | lifted_goto st i : 
       lifted_parser_expr (Parser.PGoto st i)
   | lifted_select exp default cases i: 
       lifted_expr exp -> lifted_parser_expr default -> 
-      Field.predfs_data lifted_parser_expr cases -> lifted_parser_expr (Parser.PSelect exp default cases i).
+      Field.predfs_data lifted_parser_expr cases ->
+      lifted_parser_expr (Parser.PSelect exp default cases i).
 
-  Inductive lifted_parser_state : Parser.state_block tags_t -> Prop :=
-  | lifted_parser stmt transition : 
-      lifted_stmt stmt -> lifted_parser_expr transition -> lifted_parser_state (Parser.State stmt transition).
+  Definition lifted_parser_state (stblk : Parser.state_block tags_t) : Prop :=
+    lifted_stmt (Parser.stmt stblk) /\ lifted_parser_expr (Parser.trans stblk).
     
   Local Hint Constructors lifted_parser_expr : core.
 
-  Inductive lifted_table : Control.table tags_t -> Prop :=
-  | lifted_Table keys act :
-      Forall (fun '(_, e, _) => lifted_expr e ) keys -> lifted_table (Control.Table keys act).
+  Definition lifted_table (tbl : Control.table tags_t) : Prop :=
+    Forall (fun '(_, e, _) => lifted_expr e) (Control.table_key tbl).
   
   Inductive lifted_control_Decl : Control.d tags_t -> Prop :=
   | lifted_CDAction act sig body i :
-      lifted_stmt body -> lifted_control_Decl (Control.CDAction act sig body i)
+      lifted_stmt body ->
+      lifted_control_Decl (Control.CDAction act sig body i)
   | lifted_CDTable table_name body i :
-      lifted_table body -> lifted_control_Decl (Control.CDTable table_name body i)
+      lifted_table body ->
+      lifted_control_Decl (Control.CDTable table_name body i)
   | lifted_CDSeq d1 d2 i :
-      lifted_control_Decl d1 -> lifted_control_Decl d2 -> lifted_control_Decl (Control.CDSeq d1 d2 i).
-
+      lifted_control_Decl d1 -> lifted_control_Decl d2 ->
+      lifted_control_Decl (Control.CDSeq d1 d2 i).
 
   Section HelperLemmas.
     Variable f :
@@ -434,7 +433,7 @@ Section Lifted.
   Lemma TranslateArrowE_lifted_stmt : forall (args : Expr.arrowE tags_t) env i, 
   lifted_stmt (fst (fst (TranslateArrowE args env i))).
   Proof.
-    intros args i. induction args; intro env; simpl.
+    intros [pas returns] i env; simpl.
     destruct (TranslateArgs pas i env) eqn:Hs1. destruct p. destruct returns.
     - transformExpr_destr. constructor.
       + hyp_f_equal_fst Hs1.
@@ -445,11 +444,12 @@ Section Lifted.
   Local Hint Resolve TranslateArrowE_lifted_stmt : core.
 
   Lemma TranslateArgs_lifted_expr : forall pas env i,
-  Field.predfs_data (pred_paramarg_same lifted_expr) (snd (fst (TranslateArgs pas i env))).
+      Field.predfs_data (pred_paramarg_same lifted_expr) (snd (fst (TranslateArgs pas i env))).
   Proof.
     intros pas i. induction pas; intro env; simpl.
     - constructor.
-    - destruct a. translateArgs_destr. transformExpr_destr. destruct p; unfold F.predfs_data, F.predf_data in *; 
+    - destruct a. translateArgs_destr. transformExpr_destr.
+      destruct p; unfold F.predfs_data, F.predf_data in *; 
     unravel in *; rewrite Forall_app; split; try hyp_f_equal_snd Heqp0; repeat constructor;
     simpl; unfold pred_paramarg_same, pred_paramarg; hyp_f_equal_snd Heqp1.
   Qed.
@@ -457,12 +457,13 @@ Section Lifted.
   Local Hint Resolve TranslateArgs_lifted_expr : core.
 
   Local Hint Constructors predop : core.
-  Local Hint Constructors lifted_args : core.
 
   Lemma TransformExpr_lifted_args : forall pas i (e:Expr.e tags_t) t env,
-  lifted_args (Arrow (snd (fst (TranslateArgs pas i env))) (Some (snd (fst (TransformExpr e t))))).
+      lifted_args {|paramargs:=snd (fst (TranslateArgs pas i env));
+                    rtrns:=Some (snd (fst (TransformExpr e t)))|}.
   Proof.
-    intros pas i e t env; simpl; auto. 
+    unfold lifted_args.
+    intros pas i e t env; simpl; auto.
   Qed.
 
   Local Hint Resolve TransformExpr_lifted_args : core.
@@ -471,10 +472,10 @@ Section Lifted.
   lifted_args (snd (fst (TranslateArrowE args env i))).
   Proof.
     intros [pas returns] i env; simpl.
-    destruct (TranslateArgs pas i env) eqn:Hs1. destruct p eqn:Hs2. destruct returns eqn:Hs3.
-    - transformExpr_destr.  hyp_f_equal_snd Heqp0. 
-      + hyp_f_equal_snd Hs1. 
-    - simpl. hyp_f_equal_snd Hs1.
+    destruct (TranslateArgs pas i env) eqn:Hs1;
+      destruct p eqn:Hs2; destruct returns eqn:Hs3; cbn.
+    - transformExpr_destr. hyp_f_equal_snd Heqp0. hyp_f_equal_snd Hs1.
+    - hyp_f_equal_snd Hs1. unfold lifted_args; split; cbn; auto.
   Qed.
 
   Local Hint Resolve TranslateArrowE_lifted_args : core.
@@ -586,36 +587,37 @@ Section Lifted.
 
   Local Hint Resolve TranslateParserExpr_lifted_parser_expr : core.
 
-  Lemma TranslateParserState_lifted_stmt : forall (parser_state: Parser.state_block tags_t) (env : VarNameGen.t),
-  lifted_parser_state (fst (TranslateParserState parser_state env)).
+  Lemma TranslateParserState_lifted_stmt :
+    forall (parser_state: Parser.state_block tags_t) (env : VarNameGen.t),
+      lifted_parser_state (fst (TranslateParserState parser_state env)).
   Proof.
-  intros s. induction s. intro env. simpl. translateStmt_destr. translateParserExpr_destr.
-  destruct p. simpl. repeat constructor.
-  - hyp_f_equal Heqp (fun x:(Stmt.s tags_t) => x).
-  - hyp_f_equal_fst Heqp0.
-  - hyp_f_equal_snd Heqp0.
+    intros [s e] env; simpl; translateStmt_destr; translateParserExpr_destr.
+    destruct p. simpl. unfold lifted_parser_state; split; cbn; try constructor.
+    - hyp_f_equal Heqp (fun x:(Stmt.s tags_t) => x).
+    - hyp_f_equal_fst Heqp0.
+    - hyp_f_equal_snd Heqp0.
   Qed.
 
   Local Hint Resolve TranslateParserState_lifted_stmt : core.
 
-
-  Lemma TranslateTable_lifted_stmt : forall ( t: Control.table tags_t) (env: VarNameGen.t) (i : tags_t),
-  lifted_stmt (fst (fst (TranslateTable t env i))).
+  Lemma TranslateTable_lifted_stmt :
+    forall (t: Control.table tags_t) (env: VarNameGen.t) (i : tags_t),
+      lifted_stmt (fst (fst (TranslateTable t env i))).
   Proof.
-  intros t i. induction t. intro env. simpl. fold_destr. 
+    intros [ky acts] i env; cbn; fold_destr; clear acts.
   Admitted.
 
   Local Hint Resolve TranslateTable_lifted_stmt : core.
 
   Lemma TranslateControlDecl_lifted_stmt : forall (cd : Control.d tags_t) (env : VarNameGen.t),
-  lifted_stmt (fst (fst (TranslateControlDecl cd env))).
+      lifted_stmt (fst (fst (TranslateControlDecl cd env))).
   Proof.
-  intro cd. induction cd; intro env; simpl; auto.  
-  - translateStmt_destr. auto. 
-  - simpl. translateTable_destr. hyp_f_equal_fst Heqp.
-  - repeat translateControlDecl_destr. constructor.
-    + hyp_f_equal_fst Heqp.
-    + hyp_f_equal_fst Heqp0.
+    intro cd. induction cd; intro env; simpl; auto.  
+    - translateStmt_destr. auto. 
+    - simpl. translateTable_destr. hyp_f_equal_fst Heqp.
+    - repeat translateControlDecl_destr. constructor.
+      + hyp_f_equal_fst Heqp.
+      + hyp_f_equal_fst Heqp0.
   Qed.  
   
   Local Hint Resolve TranslateControlDecl_lifted_stmt : core.
