deps/poulet4/lib/P4cub/BigStep/Semantics.v
@@ -70,7 +70,7 @@ Module Step.
   Import AllCubNotations V.ValueNotations V.LValueNotations.
 
   (** Statement signals. *)
-  Inductive signal : Type :=
+  Variant signal : Type :=
   | SIG_Cont                  (* continue *)
   | SIG_Exit                  (* exit *)
   | SIG_Rtrn (v : option V.v) (* return *)
@@ -87,14 +87,14 @@ Module Step.
 
   (** Evidence that control-flow
       is interrupted by an exit or return statement. *)
-  Inductive interrupt : signal -> Prop :=
+  Variant interrupt : signal -> Prop :=
   | interrupt_exit : interrupt SIG_Exit
   | interrupt_rtrn (vo : option V.v) : interrupt (SIG_Rtrn vo)
   | interrupt_rjct : interrupt SIG_Rjct.
   (**[]*)
 
   (** Context for statement evaluation. *)
-  Inductive ctx {tags_t : Type} : Type :=
+  Variant ctx {tags_t : Type} : Type :=
   | CAction (available_actions : @aenv tags_t)
             (available_externs : ARCH.extern_env)
   | CVoid                         (* void function *)
@@ -485,7 +485,7 @@ Module Step.
       (* Get control-plane entries. *)
       Env.find x cp = Some es ->
       (* Get appropriate table. *)
-      Env.find x ts = Some (Control.Table ky acts) ->
+      Env.find x ts = Some {|Control.table_key:=ky; Control.table_actions:=acts|} ->
       (* Evaluate key. *)
       Forall2 (fun '(_,k,_) '(v,_) => ⟨ ϵ, k ⟩ ⇓ v) ky vky ->
       (* Get action and arguments.
@@ -523,7 +523,7 @@ Module Step.
       (** Copy-in. *)
       let cls' := copy_in argsv ϵ cls in
       (* Evaluate extern method call. *)
-      disp mthd (Arrow argsv lvo) cls' pkt = (inl cls'', pkt') ->
+      disp mthd {|paramargs:=argsv; rtrns:=lvo|} cls' pkt = (inl cls'', pkt') ->
       (* Copy-out. *)
       let ϵ' := copy_out argsv cls'' ϵ in
       ⟪ pkt, fs, ϵ, c,
@@ -600,7 +600,7 @@ Module Step.
                         (Expr.t * Expr.e tags_t * Expr.matchkind))
                (actns : list (string))
                (i : tags_t) :
-      let tbl := Control.Table kys actns in
+      let tbl := {|Control.table_key:=kys; Control.table_actions:=actns|} in
       ⦉ tbls, aa, fns, cis, eis, ϵ, table t key:=kys actions:=actns @ i ⦊
         ⟱  ⦉ aa, t ↦ tbl;; tbls ⦊
   | cdbs_seq (d1 d2 : Control.d tags_t) (i : tags_t)
@@ -770,7 +770,7 @@ Module Step.
 
   (** Evaluating a parser instance. *)
   (* TODO: reject state? *)
-  Inductive parser_instance_big_step
+  Variant parser_instance_big_step
             {tags_t: Type} : pinst -> Paquet.t -> Paquet.t -> Prop :=
   | pibs (ϵ ϵ': epsilon) (fs: fenv) (pis: pienv) (eis: ARCH.extern_env)
          (pkt pkt': Paquet.t) (strt: AST.Parser.state_block tags_t)
@@ -781,7 +781,7 @@ Module Step.
   (**[]*)
 
   (** Evaluating a control instance. *)
-  Inductive control_instance_big_step
+  Variant control_instance_big_step
             {tags_t: Type} (cp: ctrl)
     : cinst -> Paquet.t -> Paquet.t -> Prop :=
   | cibs (ϵ ϵ' : epsilon) (fs : fenv)
@@ -794,7 +794,7 @@ Module Step.
   (**[]*)
   
   (** Entire program pipeline. *)
-  Inductive pipeline_big_step
+  Variant pipeline_big_step
             {tags_t: Type} (cp: ctrl) (pl: pipeline)
     : TopDecl.d tags_t -> Paquet.t -> Paquet.t -> Prop :=
   | pipebs (prog: TopDecl.d tags_t)
